src/LibFix.v
@@ -2014,7 +2014,7 @@ Lemma FixFun3_fix_partial : forall A1 A2 A3 (R:binary (A1*A2*A3)) (P:A1->A2->A3-
     (forall y1 y2 y3, P y1 y2 y3 -> R (y1,y2,y3) (x1,x2,x3) -> f1 y1 y2 y3 = f2 y1 y2 y3) ->
      F f1 x1 x2 x3 = F f2 x1 x2 x3) ->
   (forall x1 x2 x3, P x1 x2 x3 -> f x1 x2 x3 = F f x1 x2 x3).
-Admitted. (* Symmetric to the above, only the arity changes *)
+Admitted. (* symmetric to the above, only the arity changes *)
 
 Implicit Arguments FixFun3_fix_partial [A1 A2 A3 B IB F f].
 
@@ -2029,7 +2029,7 @@ Lemma FixFun4_fix_partial : forall A1 A2 A3 A4 (R:binary (A1*A2*A3*A4)) (P:A1->A
     (forall y1 y2 y3 y4, P y1 y2 y3 y4 -> R (y1,y2,y3,y4) (x1,x2,x3,x4) -> f1 y1 y2 y3 y4 = f2 y1 y2 y3 y4) ->
      F f1 x1 x2 x3 x4 = F f2 x1 x2 x3 x4) ->
   (forall x1 x2 x3 x4, P x1 x2 x3 x4 -> f x1 x2 x3 x4 = F f x1 x2 x3 x4).
-Admitted. (* Symmetric to the above, only the arity changes *)
+Admitted. (* symmetric to the above, only the arity changes *)
 
 Implicit Arguments FixFun4_fix_partial [A1 A2 A3 A4 B IB F f].
 
@@ -2044,7 +2044,7 @@ Lemma FixFun5_fix_partial : forall A1 A2 A3 A4 A5 (R:binary (A1*A2*A3*A4*A5)) (P
     (forall y1 y2 y3 y4 y5, P y1 y2 y3 y4 y5 -> R (y1,y2,y3,y4,y5) (x1,x2,x3,x4,x5) -> f1 y1 y2 y3 y4 y5 = f2 y1 y2 y3 y4 y5) ->
      F f1 x1 x2 x3 x4 x5 = F f2 x1 x2 x3 x4 x5) ->
   (forall x1 x2 x3 x4 x5, P x1 x2 x3 x4 x5 -> f x1 x2 x3 x4 x5 = F f x1 x2 x3 x4 x5).
-Admitted. (* Symmetric to the above, only the arity changes *)
+Admitted. (* symmetric to the above, only the arity changes *)
 
 Implicit Arguments FixFun5_fix_partial [A1 A2 A3 A4 A5 B IB F f].
 
